more lemmas

code/rocq/valid_state.v
@@ -81,7 +81,7 @@ Module valid_state (U:Unif).
 
   Definition is_and A := 
     match A with
-    | Bot | Top | And _ _ _ | Goal _ _ => true
+    | Bot | Top | And _ _ _ | OK => true
     | _ => false
     end.
 
@@ -91,6 +91,9 @@ Module valid_state (U:Unif).
     | _ => false
     end.
 
+  Lemma base_and_is_or {A}: base_and A -> is_or A = false.
+  Proof. case: A => //. Qed.
+
   Fixpoint valid_state s :=
     match s with
     | Goal _ _ | OK | Bot | Top => true
@@ -99,7 +102,7 @@ Module valid_state (U:Unif).
       if is_dead A then valid_state B
       else valid_state A && (bbOr B)
     | And A B0 B => 
-      [&& is_or A, valid_state A,
+      [&& is_or A, valid_state A, is_and B,
         if success A then valid_state B 
         else (B0 == B)
         (* We should notice that in (OK \/ KO) /\ OK the reset point is forced to be cut *)
@@ -119,6 +122,25 @@ Module valid_state (U:Unif).
     rewrite HA// andbF//.
   Qed.
 
+  Lemma base_and_is_and {A}: base_and A -> is_and A.
+  Proof. elim: A => //. Qed.
+
+  Lemma base_and_ko_is_and {A}: base_and_ko A -> is_and A.
+  Proof. elim: A => //. Qed.
+
+  Lemma bbAnd_is_and {A}: bbAnd A -> is_and A.
+  Proof. elim: A => //. Qed.
+
+  Lemma is_and_cutl {A}: is_and A -> is_and (cutl A).
+  Proof. elim: A => //. Qed.
+
+  Lemma is_or_cutl {A}: is_or A -> is_or (cutl A).
+  Proof. elim: A => //A HA s B HB/=; rewrite fun_if/=if_same//. Qed.
+
+  Lemma is_or_big_or {p s t}: is_or (big_or p s t).
+  Proof. rewrite /big_or; case: F => //-[]//. Qed.
+
+
   Lemma valid_state_dead1 {A} : valid_state A -> is_dead A = false.
   Proof. apply: contraPF => /valid_state_dead->//. Qed.
 
@@ -127,7 +149,7 @@ Module valid_state (U:Unif).
     elim A => //; clear => A HA B +; rewrite /base_or_aux //=; case: A HA => //.
     move=> p a _ + A + /andP [] /eqP H ; rewrite H.
     move=> _ HVA HA. rewrite (HVA HA) /=.
-    rewrite /bbAnd HA eqxx//.
+    rewrite /bbAnd HA eqxx// base_and_is_and//.
   Qed.
 
   Lemma valid_state_big_and {pr l} : valid_state (big_and pr l).
@@ -139,7 +161,7 @@ Module valid_state (U:Unif).
       apply: base_and_valid.
     elim: A=> //.
     move=> []// _ B0 HB0 B HB/=/and3P[H/eqP->]bB.
-    rewrite eqxx /bbAnd bB orbT//.
+    rewrite eqxx /bbAnd bB orbT//base_and_ko_is_and//.
   Qed.
 
   Lemma big_or_aux_not_bot {pr l rs}: big_or_aux pr l rs != Bot.
@@ -166,7 +188,7 @@ Module valid_state (U:Unif).
   Proof.
     elim: B => //.
     move=> []// HA B0 _ B HB/= /and3P[bB0 /eqP <-] H.
-    by rewrite /bbAnd ?eqxx H ?orbT.
+    rewrite eqxx /bbAnd H base_and_ko_is_and//orbT//.
   Qed.
 
   Lemma base_and_base_or_aux {A}: base_and A -> base_or_aux A.
@@ -174,21 +196,6 @@ Module valid_state (U:Unif).
 
   Lemma base_and_ko_base_or_aux_ko {A}: base_and_ko A -> base_or_aux_ko A.
   Proof. case: A => //. Qed.
-
-  Lemma base_and_is_and {A}: base_and A -> is_and A.
-  Proof. elim: A => //. Qed.
-
-  Lemma base_and_ko_is_and {A}: base_and_ko A -> is_and A.
-  Proof. elim: A => //. Qed.
-
-  Lemma is_and_cutl {A}: is_and A -> is_and (cutl A).
-  Proof. elim: A => //. Qed.
-
-  Lemma is_or_cutl {A}: is_or A -> is_or (cutl A).
-  Proof. elim: A => //A HA s B HB/=; rewrite fun_if/=if_same//. Qed.
-
-  Lemma is_or_big_or {p s t}: is_or (big_or p s t).
-  Proof. rewrite /big_or; case: F => //-[]//. Qed.
 
   Lemma bbOr_valid {B}:
     bbOr B -> valid_state B.
@@ -198,12 +205,12 @@ Module valid_state (U:Unif).
     + move=> A HA s B HB/=/andP[bA bB].
       rewrite HA ?base_and_base_or_aux// /bbOr bB HB// if_same//base_and_is_and//orbT//.
     + move=> []// p a Ha B0 HB0 B HB /=/andP[/eqP->]bB.
-      by rewrite /bbAnd eqxx bB ?(ssa_id bB).
+      rewrite eqxx base_and_is_and bB//.
     elim: B => //.
     + move=> A HA s B HB /= /andP [bA bB].
       rewrite HB//HA?base_and_ko_base_or_aux_ko// /bbOr bB orbT if_same//base_and_ko_is_and//orbT//.
     + move=> [] // HA B0 _ B HB /= /and3P[] bB0 /eqP <-.
-      rewrite /bbAnd bB0 eqxx ?orbT//.
+      rewrite /bbAnd bB0 eqxx base_and_ko_is_and// orbT//.
   Qed.
 
   Lemma base_and_base_and_ko_cut {B} : base_and B -> base_and_ko (cutr B).
@@ -307,8 +314,8 @@ Module valid_state (U:Unif).
       move=>/=/andP[vA bB]; rewrite HA// bbOr_cutr//is_dead_cutl dA//is_and_cutl//.
     move=> A HA B0 HB0 B HB /=/andP[sA sB].
     rewrite sA/=success_cut//=.
-    move=>/and4P[oA vA vB bB0].
-    rewrite is_or_cutl// HB// bbAnd_cutl//HA//.
+    move=>/and5P[oA vA aB vB bB0].
+    rewrite is_or_cutl// HB// bbAnd_cutl//HA// is_and_cutl//.
   Qed.
 
   (* Lemma simpl_valid_state_and {A B0 B}: valid_state (And A B0 B) -> 
@@ -326,6 +333,15 @@ Module valid_state (U:Unif).
     - move=> A HA s B HB s1/= _; case: ifP => dA; case: expand => //.
   Qed.
 
+  Lemma is_and_expand {s A r}: is_and A -> expand s A = r -> is_and (get_state r).
+  Proof.
+    move=> + <-; clear r. 
+    elim: A s => //.
+    move=> A HA B0 _ B HB s1/=.
+    case eA: expand => //=.
+    rewrite get_state_And//.
+  Qed.
+
   Lemma base_and_bbAnd {A}: base_and A -> bbAnd A.
   Proof. rewrite/bbAnd=>->//. Qed.
 
@@ -340,19 +356,20 @@ Module valid_state (U:Unif).
         rewrite get_state_Or/=dA IHB//.
       have /= := IHA s1 vA.
       case X: expand => //= H; rewrite (expand_not_dead dA X) H//bbOr_cutr//.
-    + move=> A HA B0 _ B HB s1 /=/and4P[oA vA].
+    + move=> A HA B0 _ B HB s1 /=/and5P[oA vA aB].
       case: ifP => [sA vB /= bB0 | sA /eqP->]/=.
         rewrite succes_is_solved//=.
         have:= HB s1 vB.
-        case X: expand => //[s2 C|s2 C|C|s2 C]/=vC; rewrite ?valid_state_cut// ?success_cut// ?sA ?vA vC//?oA//is_or_cutl// bbAnd_cutl//.
+        case X: expand => //[s2 C|s2 C|C|s2 C]/=vC; try by rewrite sA (is_and_expand aB X) vA vC oA//.
+        rewrite is_or_cutl//valid_state_cut//(is_and_expand aB X) success_cut// vC //= bbAnd_cutl//.
       case: ifP => [fA bB|fA bB].
-        rewrite failed_expand//=vA sA eqxx /= bB oA fA//.
+        rewrite failed_expand//=vA sA eqxx /= bB oA fA aB//.
       have:= HA s1 vA.
-      case X: expand => //=[|||s2 C] H; last first; [|rewrite H eqxx /bbAnd bB if_same base_and_valid//if_same (is_or_expand oA X)// ..].
+      case X: expand => //=[|||s2 C] H; last first; [|rewrite H eqxx /bbAnd bB if_same base_and_valid//if_same (is_or_expand oA X) aB//..].
       have:= HB s2 (base_and_valid bB).
       have /=oC := is_or_expand oA X.
       have [_ sC]:= expand_solved_success X.
-      case Y: expand => //= H1; rewrite ?oC?H?H1?bB?sC?(base_and_bbAnd bB)//.
+      case Y: expand => //= H1; rewrite ?oC?H?H1?bB?sC?(base_and_bbAnd bB) (is_and_expand (base_and_is_and bB) Y)//.
       rewrite is_or_cutl//valid_state_cut//success_cut//=bbAnd_cutl//base_and_bbAnd//.
   Qed.
 
@@ -464,15 +481,23 @@ Module valid_state (U:Unif).
       rewrite next_alt_aux_base_and//. 
   Qed.
 
-  Lemma is_or_next_alt {s1 A s2 B}: is_or A -> next_alt s1 A = Some (s2, B) -> is_or B.
+  Lemma is_and_or_next_alt {s1 A s2 B}: next_alt s1 A = Some (s2, B) -> ((is_or A = is_or B) * (is_and A = is_and B)).
   Proof.
     elim: A s1 s2 B => //.
-    - move=> p /= ???? _ [_<-]//.
-    - move=> A HA s B HB s1 s2 C/= _.
+    - move=> ???[_<-]//.
+    - move=> p /= ????[_<-]//.
+    - move=> A HA s B HB s1 s2 C/=.
       case:ifP => //dA.
         case: next_alt => //-[s3 D][_<-]//.
       case: next_alt => // [[s3 D][_<-]|]//.
       case: ifP => //; case: next_alt => //-[s3 D] _ [_<-]//.
+    - move=> A HA B0 _ B HB/=s1 s2 C.
+      case: ifP => //dA.
+      case: ifP => //fA.
+        case nA: next_alt => //[[]]; case: ifP => // _ [_<-]//.
+      case nB: next_alt => //[[]|].
+        move=>[_<-]//.
+      case nA: next_alt => //[[]]; case: ifP => // _ [_<-]//.
   Qed.
 
   Lemma valid_state_next_alt {s1 s2 A B}: 
@@ -493,14 +518,14 @@ Module valid_state (U:Unif).
         case Y: next_alt => [[s3 D]|]//.
         move=>[_<-]/=; rewrite is_dead_dead (HB _ _ _ _ Y)//bbOr_valid//.
       (* move=>[_<-]/=; rewrite is_dead_dead bbOr_valid//. *)
-    + move=> A HA B0 HB0 B HB s1 s2 C/=/and4P[oA vA].
+    + move=> A HA B0 HB0 B HB s1 s2 C/=/and5P[oA vA aB].
       case: ifP => /=[sA vB bB0|sA /eqP?]; subst.
         rewrite success_is_dead//success_failed//.
         case X: next_alt => [[s3 D]|].
-          move=>[_<-]/=; rewrite vA sA oA/= (HB _ _ _ vB X)//.
+          move=>[_<-]/=; rewrite vA sA oA/= (HB _ _ _ vB X)//-(is_and_or_next_alt X)aB//.
         case Y: next_alt=> [[s3 D]|]//.
         case: ifP => //fB0[_<-]/=; rewrite (HA _ _ _ vA Y)bbAnd_valid//eqxx bB0 if_same//=.
-        rewrite (is_or_next_alt oA Y).
+        rewrite -(is_and_or_next_alt Y) oA bbAnd_is_and//.
         move: bB0; rewrite /bbAnd => /orP[].
           move=>->; rewrite if_same//.
         move=>/base_and_ko_failed; rewrite fB0//.
@@ -509,13 +534,13 @@ Module valid_state (U:Unif).
       case: ifP => fA bB.
         case X: next_alt => [[s3 D]|]//.
         case: ifP => fB//[_<-]/=; rewrite (HA _ _ _ vA X)bbAnd_valid//eqxx bB if_same//.
-        rewrite (is_or_next_alt oA X).
+        rewrite -(is_and_or_next_alt X) oA bbAnd_is_and//.
         move: bB; rewrite /bbAnd => /orP[].
           move=>->; rewrite if_same//.
         move=>/base_and_ko_failed; rewrite fB//.
       rewrite (next_alt_aux_base_and bB).
       move=>[_<-]/=.
-      rewrite vA sA eqxx bB fA oA//.
+      rewrite vA sA eqxx bB fA oA// bbAnd_is_and///bbAnd bB//.
   Qed.
 
   Lemma base_and_clean_success {A}:
@@ -530,6 +555,22 @@ Module valid_state (U:Unif).
     case: A => //=-[]//=B C/and3P[bB /eqP<-].
   Qed.
 
+  Lemma is_or_clean_success {A}:
+    is_or A = is_or (clean_success A).
+  Proof.
+    elim: A => //.
+    - move=> A HA s B HB/=; rewrite fun_if if_same//.
+    - move=> A HA B0 _ B HB/=; rewrite fun_if/=if_same//.
+  Qed.
+
+  Lemma is_and_clean_success {A}:
+    is_and A = is_and (clean_success A).
+  Proof.
+    elim: A => //.
+    - move=> A HA s B HB/=; rewrite fun_if if_same//.
+    - move=> A HA B0 _ B HB/=; rewrite fun_if/=if_same//.
+  Qed.
+
   Lemma valid_state_clean_success {A}:
     valid_state A -> valid_state (clean_success A).
   Proof.
@@ -539,10 +580,10 @@ Module valid_state (U:Unif).
       case: ifP => //=.
       move=> dA/andP[vA bB].
       rewrite HA//bB bbOr_valid// if_same//.
-    - move=> A HA B0 _ B HB/=/and4P[oA vA]; rewrite (fun_if valid_state)/=oA vA.
+    - move=> A HA B0 _ B HB/=/and5P[oA vA aB]; rewrite (fun_if valid_state)/=oA vA.
       case: ifP => /=[sA vB bB0|sA /eqP->].
-        rewrite bB0 andbT; apply: HB vB.
-      rewrite eqxx//.
+        rewrite bB0 andbT -is_and_clean_success//aB; apply: HB vB.
+      rewrite eqxx//aB//.
   Qed.
 
   Lemma runP_run {s1 A s2 B}:
